some cleanup

SP1Chips/JalrChip.lean
@@ -9,38 +9,38 @@ open Sail SailState BitVec LeanRV64D.Functions
 
 variable (Main : Vector (Fin KB) 39) (s : SailState)
 
-lemma op_a_lt32_of_constraints {Main : Vector (Fin KB) 39} (h : (constraints Main).allHold)
-    (h_is_real : Main[30] = 1) : Main[6].val < 2^5 := by
-  simp only [BB_eq, Nat.reducePow]
-  have reader_cstrs := by
-    simp [SP1ConstraintList.allHold, constraints, SP1Constraint.toProp] at h
-    exact h.2.2.1
-  simp [ITypeReader.constraints, h_is_real, Opcode.ofNat,
-    Nat.ble, Nat.beq, SP1Constraint.toProp] at reader_cstrs
-  -- aesop
-  sorry
+-- lemma op_a_lt32_of_constraints {Main : Vector (Fin KB) 39} (h : (constraints Main).allHold)
+--     (h_is_real : Main[30] = 1) : Main[6].val < 2^5 := by
+--   simp only [BB_eq, Nat.reducePow]
+--   have reader_cstrs := by
+--     simp [SP1ConstraintList.allHold, constraints, SP1Constraint.toProp] at h
+--     exact h.2.2.1
+--   simp [ITypeReader.constraints, h_is_real, Opcode.ofNat,
+--     Nat.ble, Nat.beq, SP1Constraint.toProp] at reader_cstrs
+--   -- aesop
+--   sorry
 
-lemma op_b_lt32_of_constraints {Main : Vector (Fin KB) 39} (h : (constraints Main).allHold)
-    (h_is_real : Main[30] = 1) : Main[14].val < 2^5 := by
-  simp only [BB_eq, Nat.reducePow]
-  have reader_cstrs := by
-    simp [SP1ConstraintList.allHold, constraints, SP1Constraint.toProp] at h
-    exact h.2.2.1
-  simp [ITypeReader.constraints, h_is_real, Opcode.ofNat,
-    Nat.ble, Nat.beq, SP1Constraint.toProp] at reader_cstrs
-  -- aesop
-  sorry
+-- lemma op_b_lt32_of_constraints {Main : Vector (Fin KB) 39} (h : (constraints Main).allHold)
+--     (h_is_real : Main[30] = 1) : Main[14].val < 2^5 := by
+--   simp only [BB_eq, Nat.reducePow]
+--   have reader_cstrs := by
+--     simp [SP1ConstraintList.allHold, constraints, SP1Constraint.toProp] at h
+--     exact h.2.2.1
+--   simp [ITypeReader.constraints, h_is_real, Opcode.ofNat,
+--     Nat.ble, Nat.beq, SP1Constraint.toProp] at reader_cstrs
+--   -- aesop
+--   sorry
 
-def sp1_op_a (cstrs : (constraints Main).allHold) (h_is_real : Main[30] = 1) : BitVec 5 :=
-  Main[6].val#'(op_a_lt32_of_constraints cstrs h_is_real)
+def sp1_op_a (Main : Vector (Fin KB) 39) : BitVec 5 :=
+  BitVec.ofNat 5 Main[6].val
 
-def sp1_op_b (cstrs : (constraints Main).allHold) (h_is_real : Main[30] = 1): BitVec 5 :=
-  Main[14].val#'(op_b_lt32_of_constraints cstrs h_is_real)
+def sp1_op_b (Main : Vector (Fin KB) 39) : BitVec 5 :=
+  BitVec.ofNat 5 Main[14].val
 
-def sp1_op_c : BitVec 12 := BitVec.ofNat 12 Main[21].val
+def sp1_op_c (Main : Vector (Fin KB) 39) : BitVec 12 := BitVec.ofNat 12 Main[21].val
 
-def sp1_jalr  (cstrs : (constraints Main).allHold) (h_is_real : Main[30] = 1): SailM Unit := do
-  let op_a := sp1_op_a Main cstrs h_is_real
+def sp1_jalr (Main : Vector (Fin KB) 39) : SailM Unit := do
+  let op_a := sp1_op_a Main
   writeReg Register.nextPC (Word.toBitVec64 #v[Main[30], Main[31], Main[32], Main[33]])
   wX_bits (.Regidx op_a) (Word.toBitVec64 #v[Main[34], Main[35], Main[36], Main[37]])
 
@@ -52,12 +52,11 @@ set_option debug.skipKernelTC true in
 theorem JALR_correct
     (cstrs : (constraints Main).allHold)
     (h_is_real : Main[30] = 1)
-    (state_cstrs : (constraints Main).initialState s)
-    (h_misa : Register.misa ∈ s.regs) :
-    let op_b := sp1_op_b Main cstrs h_is_real
-    let op_a := sp1_op_a Main cstrs h_is_real
+    (state_cstrs : (constraints Main).initialState s) :
+    let op_b := sp1_op_b Main
+    let op_a := sp1_op_a Main
     let op_c := sp1_op_c Main
-    (spec_jalr op_c (.Regidx op_b) (.Regidx op_a)).run s = (sp1_jalr Main cstrs h_is_real).run s := by
+    (spec_jalr op_c (.Regidx op_b) (.Regidx op_a)).run s = (sp1_jalr Main).run s := by
   extract_lets op_c op_b op_a
 
   -- pull out state constraints about the contents of register and pc reads
@@ -69,6 +68,7 @@ theorem JALR_correct
   obtain ⟨res_cstrs, ⟨pc_cstrs, ⟨reader_cstrs, ⟨inc_pc_cstrs, chip_cstrs⟩⟩⟩⟩ := cstrs
 
   simp [ITypeReader.constraints, h_is_real, Opcode.ofNat, Nat.ble, Nat.beq, SP1Constraint.toProp] at reader_cstrs
+
   stop
   obtain ⟨⟨h_op_b, h_c_sign_extend⟩, ⟨h_op_a, ⟨_, ⟨⟨h_c_0, ⟨h_c_1, ⟨h_c_2, h_c_3⟩⟩⟩, ⟨op_a_0_is_bool, ⟨op_a_0_iff_op_a_is_0, ⟨pc_mul_4, ⟨h_pc_0, ⟨h_pc_1, h_pc_2⟩⟩⟩⟩⟩⟩⟩⟩⟩ := reader_cstrs.1
   let read_op_b' := read_op_b h_op_b
